%!TEX TS-program = xelatex
%!TEX encoding = UTF-8 Unicode

\documentclass[a4paper]{article}

\usepackage{xltxtra}
\usepackage{amsfonts}
\usepackage{polyglossia}
\usepackage{fancyhdr}
\usepackage{geometry}
\usepackage{dsfont}
\usepackage{amsmath}
\usepackage{amsthm}
\usepackage{amssymb}
\usepackage{physics}
\usepackage[shortlabels]{enumitem}

\geometry{a4paper,left=15mm,right=15mm,top=20mm,bottom=20mm}
\pagestyle{fancy}
\lhead{Devon Morris}
\chead{Differential Geometry - Homework 4}
\rhead{\today}
\cfoot{\thepage}

\setlength{\headheight}{23pt}
\setlength{\parindent}{0.0in}
\setlength{\parskip}{0.0in}

\newtheorem*{prop}{Proposition}
\newtheorem*{defn}{Definition}
\begin{document}

\section*{Problem 1}%
Let $X,Y,Z \in \Gamma^{\infty}(TM)$ be smooth vector fields, and $f,g \in C^{\infty}(M)$ be smooth functions. Prove the following:
\begin{enumerate}[(a)]
  \item Jacobi's identity: $[[X,Y],Z] + [[Y,Z],X] + [[Z,X],Y] = 0$
  \item $[fX,gY] = fg[X,Y] + fX(g)Y - gY(f)X$
\end{enumerate}

\begin{proof}
  We will use the definition $[X,Y](f) = X(Y(f)) - Y(X(f))$ instead of coordinate definitions.
  \begin{enumerate}[(a)]
    \item Consider $[[X,Y],Z] + [[Y,Z],X] + [[Z,X],Y]$, using the definition of the lie bracket and linearity of vector fields on functions,
      \[
        \begin{aligned}
          ([[X,Y]&,Z] + [[Y,Z],X] + [[Z,X],Y])(f)\\ 
          =& [X,Y](Z(f)) - Z([X,Y](f)) + [Y,Z](X(f)) - X([Y,Z](f)) + [Z,X](Y(f)) - Y([Z,X](f)) \\
          =& X(Y(Z(f)) - Y(X(Z(f))) - Z(X(Y(f)) - Y(X(f))) + Y(Z(X(f))) - Z(Y(X(f))) \\
           &- X(Y(Z(f)) - Z(Y(f))) + Z(X(Y(f))) - X(Z(Y(f))) - Y(Z(X(f)) - X(Z(f))) \\
          =& X(Y(Z(f)) - Y(X(Z(f))) - Z(X(Y(f))) + Z(Y(X(f))) + Y(Z(X(f))) - Z(Y(X(f))) \\
           & -X(Y(Z(f))) + X(Z(Y(f))) + Z(X(Y(f))) - X(Z(Y(f))) -Y(Z(X(f))) - Y(X(Z(f))) \\
          =& 0 
        \end{aligned}
      \]
      Since this holds for arbitrary functions $f \in C^{\infty}(M)$, we have
      \[
        [[X,Y],Z] + [[Y,Z],X] + [[Z,X],Y] = 0
      \]
    \item Let $h \in C^{\infty}(M)$. Thinking of these tangent vectors as derivations we recall that $X(fg) = gX(f) + fX(g)$, since it must satisfy Leibniz identity. We can think of $X(f) \in C^{\infty}(M)$, using these properties we have
      \[
        \begin{aligned}
          \left[ f X , g Y \right](h) &= fX(gY(h)) - gY(fX(h)) \\
                                      &= fX(g)Y(h) + fgX(Y(h)) - gX(h)Y(f) - gfY(X(h)) \\
                                      &= fg[X,Y](h) + fX(g)Y(h) - gY(f)X(h)
        \end{aligned}
      \]
      Since $h$ is an arbitrary smooth function we have
      \[[fX,gY] = fg[X,Y] + fX(g)Y - gY(f)X
      \]
  \end{enumerate}
\end{proof}


\end{document}
