%!TEX TS-program = xelatex
%!TEX encoding = UTF-8 Unicode

\documentclass[a4paper]{article}

\usepackage{xltxtra}
\usepackage{amsfonts}
\usepackage{polyglossia}
\usepackage{fancyhdr}
\usepackage{geometry}
\usepackage{dsfont}
\usepackage{amsmath}
\usepackage{amsthm}
\usepackage{physics}
\usepackage{float}
\usepackage{tikz}
\usepackage{bm}
\usepackage[shortlabels]{enumitem}
\usetikzlibrary{shapes,arrows,positioning}

\geometry{a4paper,left=15mm,right=15mm,top=20mm,bottom=20mm}
\pagestyle{fancy} \lhead{Devon Morris}
\chead{Detection \& Estimation Theory - Homework 6}
\rhead{\today}
\cfoot{\thepage}

\setlength{\headheight}{23pt}
\setlength{\parindent}{0.0in}
\setlength{\parskip}{0.0in}

\newtheorem{prop}{Proposition}
\newtheorem*{sol}{Solution}

\tikzset{
block/.style = {draw, fill=white, rectangle, minimum height=3em, minimum width=3em},
tmp/.style  = {coordinate}, 
sum/.style= {draw, fill=white, circle, node distance=1cm},
input/.style = {coordinate},
output/.style= {coordinate},
pinstyle/.style = {pin edge={to-,thin,black}
}
}
\DeclareMathOperator*{\argmax}{arg\,max}
\DeclareMathOperator*{\argmin}{arg\,min}

\begin{document}
\section*{Problem 1}
Let $N[0,t)$ denote the number of particles emitted from a radioactive source on the time interval $[0,t)$. This is a Poisson random variable
\[
  P[N[0,t) = n] = e^{-\lambda t}\frac{(\lambda t)^n}{n!}
\]
\[
  EN[0,t) = \lambda t; \quad \text{var}N[0,t) = \lambda t
\]
Let $(t_1, t_2, \dots, t_n)$ denote a sequence of times at which $N[0,t)$ is measured.
\begin{enumerate}
  \item Find the MMSE estimator of $N[0,t_n)$, given $N[0,t_i)$, $i=1,2, \dots, n-1$
  \item Find mean of the MMSE estimator.
  \item Find the mean-squared error the MMSE estimator.
\end{enumerate}

\begin{proof}[Solution]
  \begin{enumerate}
    \item To avoid cumbersome notation, I'm going to use $t_i$ and $N[0,t_i)$ synonomously. Since we want the MMSE estimator we can simply calculate
      \[
        t_{nB} = E[t_n|t_1, \dots, t_{n-1}]
      \]
      To find this, we first need $P[N[0,t) = k | t_1, \dots, t_{n-1}]$. It should be straightforward to see that
      \[
        P[t_1 = k_1, \dots, t_n = k_n] = \prod_{i=0}^n e^{-\lambda (t_i - t_{i-1})} \frac{(\lambda(t_i - t_{i-1}))^{k_i - k_{i-1}}}{(k_i - k_{i-1})!}
      \]
      i.e. these random variables are still independent over the intervals between $t_i - t_{i-1}$. This implies that $t_0 = 0$ and $k_0 = 0$.
      \[
        \begin{aligned}
          P[t_1 = k_1, \dots, t_n = k_n] &= e^{-\lambda t_n}\lambda^{k_n} \prod_{i=0}^n  \frac{(t_i - t_{i-1})^{k_i-k_{i-1}}}{(k_i - k_{i-1})!} \\
        \end{aligned}
      \]
      However this implies that,
      \[
        P[t_1 = k_1, \dots, t_{n-1} = k_{n-1}] = e^{-\lambda t_{n-1}} \lambda^{k_{n-1}} \prod_{i=0}^{n-1}  \frac{(t_i - t_{i-1})^{k_i-k_{i-1}}}{(k_i - k_{i-1})!} \\
      \]
      So we have that 
      \[
        P[t_n = k_n| t_1 = k_1, \dots, t_{n-1} = k_{n-1}] =  e^{-\lambda(t_n - t_{n-1})} \frac{(\lambda(t_n - t_{n-1}))^{k_n - k_{n-1}}}{(k_n - k_{n-1})!}
      \]
      Which makes sense because $t_1, \dots, t_{n-2}$ contain redundant information. So now consider the random variable $t_n' = t_n - k_{n-1}$, which gives us
      \[
        P[t_n' = k_n] = P[t_n - k_{n-1} = k_n] = P[t_n = k_n + k_{n-1}] = e^{-\lambda (t_n - t_{n-1})} \frac{(\lambda(t_n - t_{n-1}))^{k_n}}{k_n!}
      \]
      which is poisson distributed and has mean $E t_n' = \lambda(t_n - t_{n-1})$, so we have that
      \[
        t_nB = \lambda(t_n - t_{n-1}) + k_{n-1}
      \]
      which totally makes sense.

  \end{enumerate}
\end{proof}

\end{document}
